src/Ex/RuleTransformOk.v
@@ -1,0 +1,1050 @@
+Require Import Bool Vector List String Peano_dec Lia.
+Require Import Common FMap HVector IndexSupport Syntax Semantics StepM Invariant Simulation.
+Require Import Topology RqRsTopo.
+Require Import RqRsLang.
+
+Import PropMonadNotations.
+
+Require Import Ex.Template Ex.RuleTransform.
+
+Set Implicit Arguments.
+
+Local Open Scope list.
+Local Open Scope hvec.
+Local Open Scope fmap.
+
+Lemma concat_map_In:
+  forall {A} (a: A) l,
+    In a l ->
+    forall {B} (f: A -> B) (g: A -> list B),
+      (forall a, In (f a) (g a)) ->
+      In (f a) (List.concat (map g l)).
+Proof.
+  induction l; simpl; intros; auto.
+  destruct H; subst.
+  - apply in_or_app; left; auto.
+  - apply in_or_app; right; auto.
+Qed.
+
+Section RssHolderOk.
+  Variable (tr: tree).
+  Hypothesis (Htr: tr <> Node nil).
+  Context `{dv:DecValue} `{oifc: OStateIfc}.
+
+  Local Notation topo := (fst (tree2Topo tr 0)).
+  Local Notation cifc := (snd (tree2Topo tr 0)).
+
+  Variables (impl spec: System).
+
+  (** Required invariants *)
+
+  Definition RssWf (oidx: IdxT) (rss: list (IdxT * option Msg)) :=
+    SubList (map fst rss) (sys_minds impl ++ sys_merqs impl) /\
+    NoDup (map fst rss) /\
+    Forall (fun iom =>
+              exists cidx,
+                parentIdxOf topo cidx = Some oidx /\
+                rsUpFrom cidx = fst iom) rss /\
+    Forall (fun iom =>
+              match snd iom with
+              | Some rs => rs.(msg_type) = MRs
+              | None => True
+              end) rss.
+
+  Definition RssWfORq (oidx: IdxT) (orq: ORq Msg) :=
+    orq@[downRq] >>=[True]
+       (fun rqid =>
+          RssWf oidx rqid.(rqi_rss) /\
+          (rqid.(rqi_midx_rsb)
+                  >>=[True] (fun rsb => forall oidx, rsb <> rsUpFrom oidx))).
+
+  Definition RssWfInv (st: State) :=
+    forall oidx, (st_orqs st)@[oidx] >>=[True] (fun orq => RssWfORq oidx orq).
+
+  (** End of the invariants *)
+
+  Definition RssORqEquiv (orq1 orq2: ORq Msg) :=
+    orq1@[upRq] = orq2@[upRq] /\
+    (orq1@[downRq] = None -> orq2@[downRq] = None) /\
+    (forall rqid1,
+        orq1@[downRq] = Some rqid1 ->
+        exists rqid2,
+          orq2@[downRq] = Some rqid2 /\
+          rqid1.(rqi_msg) = rqid2.(rqi_msg) /\
+          map fst rqid1.(rqi_rss) = map fst rqid2.(rqi_rss) /\
+          rqid1.(rqi_midx_rsb) = rqid2.(rqi_midx_rsb)).
+
+  Definition RssEquivPrec (prec: OPrec) :=
+    forall ost orq1 mins,
+      prec ost orq1 mins ->
+      forall orq2,
+        RssORqEquiv orq1 orq2 -> prec ost orq2 mins.
+
+  Definition RssEquivTrs (trs: OTrs) :=
+    forall ost orq1 mins nost norq1 mouts,
+      trs ost orq1 mins = (nost, norq1, mouts) ->
+      forall orq2,
+        RssORqEquiv orq1 orq2 ->
+        exists norq2,
+          trs ost orq2 mins = (nost, norq2, mouts) /\
+          RssORqEquiv norq1 norq2.
+
+  Definition NoRsUpInputs (mins: list (Id Msg)) :=
+    forall idm,
+      In idm mins ->
+      (exists oidx, idOf idm = rqUpFrom oidx \/ idOf idm = downTo oidx).
+
+  Definition NoRsUpInputsPrec (prec: OPrec) :=
+    forall ost orq mins, prec ost orq mins -> NoRsUpInputs mins.
+
+  Definition NoRssChange (orq1 orq2: ORq Msg) :=
+    match orq1@[downRq], orq2@[downRq] with
+    | Some rqid1, Some rqid2 => rqid1.(rqi_rss) = rqid2.(rqi_rss)
+    | Some rqid1, None => Forall (fun rs => snd rs = None) rqid1.(rqi_rss)
+    | None, Some rqid2 => Forall (fun rs => snd rs = None) rqid2.(rqi_rss)
+    | None, None => True
+    end.
+
+  Definition NoRssChangeTrs (trs: OTrs) :=
+    forall ost orq mins nost norq mouts,
+      trs ost orq mins = (nost, norq, mouts) ->
+      NoRssChange orq norq.
+
+  Definition RssEquivRule (rule: Rule) :=
+    RssEquivPrec (rule_precond rule) /\ RssEquivTrs (rule_trs rule) /\
+    NoRsUpInputsPrec (rule_precond rule) /\
+    NoRssChangeTrs (rule_trs rule).
+
+  Definition ImplRulesR (oidx: IdxT) (rule: Rule) :=
+    (RssEquivRule rule) \/
+    (exists ridx msgId rqId prec trs, rule = rsRelease ridx msgId rqId prec trs) \/
+    (exists ridx msgId rqId cidx,
+        parentIdxOf topo cidx = Some oidx /\
+        rule = rsTakeOne ridx msgId rqId cidx).
+
+  Definition ImplRules :=
+    forall iobj,
+      In iobj impl.(sys_objs) ->
+      (forall rule, In rule iobj.(obj_rules) -> ImplRulesR iobj.(obj_idx) rule) /\
+      (forall ridx1 msgId1 cidx1 ridx2 msgId2 cidx2 rqId,
+          In (rsTakeOne ridx1 msgId1 rqId cidx1) iobj.(obj_rules) ->
+          In (rsTakeOne ridx2 msgId2 rqId cidx2) iobj.(obj_rules) ->
+          msgId1 = msgId2).
+
+  Definition SpecRulesInR (oidx: IdxT) (irules srules: list Rule) :=
+    forall rule,
+      (In rule irules ->
+       RssEquivRule rule ->
+       In rule srules) /\
+      (forall ridx msgId rqId prec trs,
+          In (rsRelease ridx msgId rqId prec trs) irules ->
+          In (rsUpRule ridx~>1 msgId rqId prec trs) srules).
+
+  Definition SpecRulesIn :=
+    forall iobj,
+      In iobj impl.(sys_objs) ->
+      exists sobj,
+        In sobj spec.(sys_objs) /\
+        iobj.(obj_idx) = sobj.(obj_idx) /\
+        SpecRulesInR iobj.(obj_idx) iobj.(obj_rules) sobj.(obj_rules).
+
+  Hypotheses (Hir: ImplRules) (Hsr: SpecRulesIn).
+
+  Section SimRssMP.
+
+    Fixpoint findRs (midx: IdxT) (rss: list (IdxT * option Msg)): option Msg :=
+      match rss with
+      | nil => None
+      | (rmidx, rmsg) :: rss' =>
+        if idx_dec rmidx midx then rmsg else findRs midx rss'
+      end.
+
+    Definition SimRssMP (iorqs: ORqs Msg)
+               (imsgs: MessagePool Msg) (smsgs: MessagePool Msg) :=
+      forall midx,
+        (forall oidx,
+            midx = rqUpFrom oidx ->
+            (* rqEdgeUpFrom topo oidx = Some midx -> *)
+            findQ midx imsgs = findQ midx smsgs) /\
+        (forall oidx,
+            midx = downTo oidx ->
+            (* edgeDownTo topo oidx = Some midx -> *)
+            findQ midx imsgs = findQ midx smsgs) /\
+        (forall oidx,
+            midx = rsUpFrom oidx ->
+            (* rsEdgeUpFrom topo oidx = Some midx -> *)
+            forall pidx,
+              In pidx (c_li_indices cifc ++ c_l1_indices cifc) ->
+              parentIdxOf topo oidx = Some pidx ->
+              ((iorqs@[pidx])
+                 >>= (fun porq =>
+                        porq@[downRq]
+                            >>= (fun rqid =>
+                                   findRs midx (rqi_rss rqid))))
+                ::> (findQ midx imsgs) = findQ midx smsgs).
+
+  End SimRssMP.
+
+  Section SimRssORqs.
+
+    Definition SimRssORqs (orqs1 orqs2: ORqs Msg) :=
+      Forall
+        (fun oidx =>
+           (forall orq1,
+               orqs1@[oidx] = Some orq1 ->
+               exists orq2,
+                 orqs2@[oidx] = Some orq2 /\
+                 RssORqEquiv orq1 orq2))
+        (c_li_indices cifc ++ c_l1_indices cifc).
+
+  End SimRssORqs.
+
+  Local Definition sim (ist: State) (sst: State): Prop :=
+    st_oss ist = st_oss sst /\
+    SimRssORqs (st_orqs ist) (st_orqs sst) /\
+    SimRssMP (st_orqs ist) (st_msgs ist) (st_msgs sst).
+
+  Definition implORqsInit: ORqs Msg :=
+    initORqs (cifc.(c_li_indices) ++ cifc.(c_l1_indices)).
+
+  Hypotheses (Hsi: impl.(sys_oss_inits) = spec.(sys_oss_inits))
+             (Hoii: impl.(sys_orqs_inits) = implORqsInit)
+             (Hosi: spec.(sys_orqs_inits) = implORqsInit).
+
+  Lemma mesi_rss_sim_init: sim (initsOf impl) (initsOf spec).
+  Proof.
+    red; repeat ssplit.
+    - assumption.
+    - red; apply Forall_forall; intros oidx ?.
+      simpl; rewrite Hoii, Hosi.
+      unfold implORqsInit; intros.
+      rewrite initORqs_value in H0 by assumption.
+      inv H0.
+      exists [].
+      rewrite initORqs_value by assumption.
+      repeat split.
+      mred.
+    - red; simpl; intros; repeat split.
+      simpl; rewrite Hoii; intros.
+      unfold implORqsInit; rewrite initORqs_value by assumption.
+      simpl; mred.
+  Qed.
+
+  Lemma mesi_rss_sim_silent:
+    forall ist sst1,
+      sim ist sst1 ->
+      exists slbl sst2,
+        getLabel RlblEmpty = getLabel slbl /\
+        step_m spec sst1 slbl sst2 /\ sim ist sst2.
+  Proof.
+    simpl; intros.
+    exists RlblEmpty; eexists.
+    repeat ssplit; eauto.
+    constructor.
+  Qed.
+
+  Hypotheses (Hierqs: impl.(sys_merqs) = cifc.(c_merqs))
+             (Hserqs: spec.(sys_merqs) = cifc.(c_merqs))
+             (Hierss: impl.(sys_merss) = cifc.(c_merss))
+             (Hserss: spec.(sys_merss) = cifc.(c_merss))
+             (Himinds: impl.(sys_minds) = cifc.(c_minds))
+             (Hsminds: spec.(sys_minds) = cifc.(c_minds))
+             (Hoinds: map obj_idx (sys_objs impl) =
+                      c_li_indices cifc ++ c_l1_indices cifc).
+
+  Lemma findQ_enqMsgs_eq:
+    forall midx (msgs1 msgs2: MessagePool Msg),
+      findQ midx msgs1 = findQ midx msgs2 ->
+      forall nmsgs,
+        findQ midx (enqMsgs nmsgs msgs1) = findQ midx (enqMsgs nmsgs msgs2).
+  Proof.
+    intros.
+    generalize dependent msgs1.
+    generalize dependent msgs2.
+    induction nmsgs as [|[nmidx nmsg] ?]; simpl; intros; [assumption|].
+    apply IHnmsgs.
+    destruct (idx_dec midx nmidx); subst.
+    - rewrite !findQ_In_enqMP; congruence.
+    - rewrite !findQ_not_In_enqMP by assumption; assumption.
+  Qed.
+
+  Lemma rsUpFrom_not_In_c_merqs:
+    forall oidx, ~ In (rsUpFrom oidx) (c_merqs cifc).
+  Proof.
+    intros.
+    unfold implORqsInit in *.
+    rewrite c_merqs_l1_rqUpFrom.
+    intro Hx.
+    apply in_map_iff in Hx; dest.
+    discriminate.
+  Qed.
+
+  Lemma rsUpFrom_not_In_c_merss:
+    forall oidx, ~ In (rsUpFrom oidx) (c_merss cifc).
+  Proof.
+    intros.
+    unfold implORqsInit in *.
+    rewrite c_merss_l1_downTo.
+    intro Hx.
+    apply in_map_iff in Hx; dest.
+    discriminate.
+  Qed.
+
+  Lemma SimRssMP_enqMsgs:
+    forall iorqs imsgs smsgs,
+      SimRssMP iorqs imsgs smsgs ->
+      forall nmsgs,
+        SimRssMP iorqs (enqMsgs nmsgs imsgs) (enqMsgs nmsgs smsgs).
+  Proof.
+    unfold SimRssMP; intros.
+    specialize (H midx); dest.
+    repeat split; intros.
+    - specialize (H _ H2); apply findQ_enqMsgs_eq; auto.
+    - specialize (H0 _ H2); apply findQ_enqMsgs_eq; auto.
+    - specialize (H1 _ H2 _ H3 H4).
+      destruct iorqs@[pidx] as [porq|]; simpl in *;
+        [destruct porq@[downRq] as [rqid|]; simpl in *|].
+      2-3: apply findQ_enqMsgs_eq; assumption.
+      clear -H1.
+      generalize dependent imsgs.
+      generalize dependent smsgs.
+      induction nmsgs as [|[nmidx nmsg] nmsgs]; simpl; intros; [assumption|].
+      apply IHnmsgs.
+      destruct (idx_dec midx nmidx); subst.
+      + rewrite !findQ_In_enqMP.
+        destruct (findRs _ _); simpl in *.
+        * rewrite app_comm_cons; congruence.
+        * congruence.
+      + rewrite !findQ_not_In_enqMP by assumption.
+        assumption.
+  Qed.
+
+  Lemma SimRssMP_enqMP:
+    forall iorqs imsgs smsgs,
+      SimRssMP iorqs imsgs smsgs ->
+      forall midx msg,
+        SimRssMP iorqs (enqMP midx msg imsgs) (enqMP midx msg smsgs).
+  Proof.
+    intros.
+    eapply SimRssMP_enqMsgs with (nmsgs := [(_, _)]) in H.
+    simpl in H; eassumption.
+  Qed.
+
+  Lemma SimRssMP_deqMsgs:
+    forall iorqs imsgs smsgs,
+      SimRssMP iorqs imsgs smsgs ->
+      forall rmsgs,
+        NoRsUpInputs rmsgs ->
+        SimRssMP iorqs (deqMsgs (idsOf rmsgs) imsgs) (deqMsgs (idsOf rmsgs) smsgs).
+  Proof.
+    red; intros.
+    specialize (H midx); dest.
+    repeat split.
+    + intros; specialize (H _ H3).
+      apply findQ_deqMsgs_eq; assumption.
+    + intros; specialize (H1 _ H3).
+      apply findQ_deqMsgs_eq; assumption.
+    + intros; specialize (H2 _ H3 _ H4 H5).
+      destruct iorqs@[pidx] as [porq|]; simpl in *;
+        [destruct porq@[downRq] as [rqid|]; simpl in *|].
+      2-3: apply findQ_deqMsgs_eq; assumption.
+      rewrite !findQ_not_In_deqMsgs
+        by (intro Hx; subst;
+            apply in_map_iff with (f:= idOf) in Hx; dest;
+            specialize (H0 _ H6); dest;
+            destruct H0; rewrite H0 in H3; discriminate).
+      assumption.
+  Qed.
+
+  Lemma SimRssMP_NoRsUpInputs_first:
+    forall mins,
+      NoRsUpInputs mins ->
+      forall imsgs,
+        Forall (FirstMPI imsgs) mins ->
+        forall iorqs smsgs,
+          SimRssMP iorqs imsgs smsgs ->
+          Forall (FirstMPI smsgs) mins.
+  Proof.
+    intros.
+    rewrite Forall_forall in H0.
+    apply Forall_forall; intros [midx msg] ?.
+    specialize (H0 _ H2).
+    eapply findQ_eq_FirstMPI; [eassumption|].
+    specialize (H1 midx); dest.
+    specialize (H _ H2); simpl in H.
+    destruct H as [oidx [|]]; subst; eauto.
+  Qed.
+
+  Lemma findRs_rss_None:
+    forall rss,
+      Forall (fun rs => snd rs = None) rss ->
+      forall midx, findRs midx rss = None.
+  Proof.
+    induction rss as [|[rmidx rs] rss]; simpl; intros; [reflexivity|].
+    inv H; simpl in *; subst.
+    destruct (idx_dec rmidx midx); auto.
+  Qed.
+
+  Lemma findRs_rs:
+    forall rss,
+      NoDup (map fst rss) ->
+      forall nmidx ors,
+        In (nmidx, ors) rss ->
+        findRs nmidx rss = ors.
+  Proof.
+    induction rss as [|[rmidx rs]]; simpl; intros; [exfalso; auto|].
+    destruct H0.
+    - inv H0; destruct (idx_dec nmidx nmidx); [reflexivity|exfalso; auto].
+    - destruct (idx_dec rmidx nmidx); subst.
+      + exfalso.
+        inv H; apply in_map with (f:= fst) in H0; auto.
+      + inv H; auto.
+  Qed.
+
+  Lemma SimRssMP_ORqs_change_silent:
+    forall iorqs imsgs smsgs,
+      SimRssMP iorqs imsgs smsgs ->
+      forall oidx porq,
+        iorqs@[oidx] = Some porq ->
+        forall norq,
+          NoRssChange porq norq ->
+          SimRssMP iorqs+[oidx <- norq] imsgs smsgs.
+  Proof.
+    unfold SimRssMP; intros.
+    specialize (H midx); dest.
+    repeat split.
+    - intros; specialize (H _ H4); assumption.
+    - intros; specialize (H2 _ H4); assumption.
+    - intros; specialize (H3 _ H4 _ H5 H6).
+      mred; simpl in *.
+      red in H1.
+      destruct porq@[downRq] as [prqid|];
+        destruct norq@[downRq] as [nrqid|]; simpl in *.
+      + congruence.
+      + rewrite findRs_rss_None in H3 by assumption.
+        assumption.
+      + rewrite findRs_rss_None by assumption.
+        assumption.
+      + assumption.
+  Qed.
+
+  Lemma mesi_rss_sim_ext_in:
+    forall oss orqs msgs sst1,
+      sim {| st_oss := oss; st_orqs := orqs; st_msgs := msgs |} sst1 ->
+      forall eins,
+        eins <> nil -> ValidMsgsExtIn impl eins ->
+        exists slbl sst2,
+          getLabel (RlblIns eins) = getLabel slbl /\
+          step_m spec sst1 slbl sst2 /\
+          sim {| st_oss := oss;
+                 st_orqs := orqs;
+                 st_msgs := enqMsgs eins msgs |} sst2.
+  Proof.
+    destruct sst1 as [soss1 sorqs1 smsgs1]; simpl; intros.
+    red in H; simpl in *; dest; subst.
+    exists (RlblIns eins); eexists.
+    repeat ssplit.
+    - reflexivity.
+    - eapply SmIns; eauto.
+      red in H1; red; congruence.
+    - red; repeat ssplit; simpl; [reflexivity|assumption|].
+      apply SimRssMP_enqMsgs; assumption.
+  Qed.
+
+  Lemma mesi_rss_sim_ext_out:
+    forall oss orqs msgs sst1,
+      sim {| st_oss := oss; st_orqs := orqs; st_msgs := msgs |} sst1 ->
+      forall eouts: list (Id Msg),
+        eouts <> nil ->
+        Forall (FirstMPI msgs) eouts ->
+        ValidMsgsExtOut impl eouts ->
+        exists slbl sst2,
+          getLabel (RlblOuts eouts) = getLabel slbl /\
+          step_m spec sst1 slbl sst2 /\
+          sim {| st_oss := oss;
+                 st_orqs := orqs;
+                 st_msgs := deqMsgs (idsOf eouts) msgs |} sst2.
+  Proof.
+    destruct sst1 as [soss1 sorqs1 smsgs1]; simpl; intros.
+    red in H; simpl in *; dest; subst.
+    assert (NoRsUpInputs eouts) as Hnrs.
+    { red; intros.
+      apply in_map with (f:= idOf) in H; apply H2 in H; simpl in H.
+      rewrite Hierss in H.
+      rewrite c_merss_l1_downTo in H.
+      apply in_map_iff in H; dest; subst.
+      eauto.
+    }
+    exists (RlblOuts eouts); eexists.
+    repeat ssplit.
+    - reflexivity.
+    - eapply SmOuts with (msgs0:= smsgs1); eauto.
+      + eapply SimRssMP_NoRsUpInputs_first; try eassumption.
+      + destruct H2.
+        split; [|assumption].
+        rewrite Hierss in H.
+        rewrite Hserss.
+        assumption.
+    - red; repeat ssplit; simpl; [reflexivity|assumption|].
+      apply SimRssMP_deqMsgs; assumption.
+  Qed.
+
+  Lemma SimRssORqs_next_ord:
+    forall orqs1 orqs2,
+      SimRssORqs orqs1 orqs2 ->
+      forall orq1 orq2,
+        RssORqEquiv orq1 orq2 ->
+        forall oidx,
+          SimRssORqs (orqs1 +[oidx <- orq1]) (orqs2 +[oidx <- orq2]).
+  Proof.
+    unfold SimRssORqs; intros.
+    apply Forall_forall; intros.
+    rewrite Forall_forall in H.
+    specialize (H _ H1).
+    destruct (idx_dec oidx x); subst.
+    all: mred; eauto.
+  Qed.
+
+  Lemma RssFullWithId_spec:
+    forall oidx orq,
+      RssWfORq oidx orq ->
+      forall msgId ost mins,
+        RssFullWithId msgId ost orq mins ->
+        exists rqid,
+          orq@[downRq] = Some rqid /\
+          exists rss,
+            rqid.(rqi_rss) = map (fun idm => (idOf idm, Some (valOf idm))) rss /\
+            Forall (fun idm => msg_id (valOf idm) = msgId) rss /\
+            ValidMsgsIn impl rss /\
+            rss = getRss orq.
+  Proof.
+    unfold RssFullWithId, getRss; intros.
+    red in H.
+    destruct orq@[downRq] as [rqid|]; simpl in *; [dest|exfalso; auto].
+    clear H1; red in H; dest.
+    exists rqid; repeat split.
+    clear -H H0 H1 H2; induction (rqi_rss rqid) as [|[rmidx rs] rss].
+    - exists nil; repeat split; [constructor|apply SubList_nil|constructor].
+    - simpl in *.
+      apply SubList_cons_inv in H; dest.
+      inv H0; inv H1; inv H2.
+      simpl in *; destruct rs as [rs|]; [|exfalso; auto].
+      specialize (IHrss H3 H8 H9 H7).
+      destruct IHrss as [prss [? [? [? ?]]]]; subst.
+      eexists ((rmidx, rs) :: _); simpl.
+      repeat split.
+      + constructor; [reflexivity|assumption].
+      + simpl; apply SubList_cons; [assumption|apply H2].
+      + red; simpl; constructor.
+        * clear -H5; intro Hx; elim H5; clear H5.
+          induction prss as [|[prmidx prs]]; simpl; intros; [elim Hx|].
+          simpl in Hx; destruct Hx; subst; auto.
+        * apply H2.
+      + congruence.
+  Qed.
+
+  Lemma RssORqEquiv_addRs:
+    forall orq1 orq2,
+      RssORqEquiv orq1 orq2 ->
+      forall midx rs,
+        RssORqEquiv (addRs orq1 midx rs) orq2.
+  Proof.
+    unfold RssORqEquiv; intros; dest.
+    repeat split.
+    - unfold addRs.
+      destruct orq1@[downRq] as [rqid1|]; simpl in *; [mred|assumption].
+    - unfold addRs.
+      destruct orq1@[downRq] as [rqid1|] eqn:Hrqid1; simpl in *; mred.
+    - unfold addRs; intros.
+      destruct orq1@[downRq] as [prqid1|] eqn:Hprqid1; simpl in *; [|mred].
+      mred; simpl.
+      specialize (H1 _ eq_refl).
+      destruct H1 as [rqid2 ?]; dest.
+      exists rqid2; repeat split; try assumption.
+      rewrite <-H3.
+      clear; induction (rqi_rss prqid1) as [|[rmidx irs]]; [reflexivity|].
+      simpl; destruct (idx_dec midx rmidx).
+      all: simpl; congruence.
+  Qed.
+
+  Lemma SimRssORqs_addRs:
+    forall orqs1 orqs2,
+      SimRssORqs orqs1 orqs2 ->
+      forall roidx porq midx rs,
+        orqs1@[roidx] = Some porq ->
+        SimRssORqs (orqs1+[roidx <- addRs porq midx rs]) orqs2.
+  Proof.
+    unfold SimRssORqs; intros.
+    rewrite Forall_forall in H.
+    apply Forall_forall; intros oidx ? ? ?.
+    specialize (H _ H1).
+    destruct (idx_dec oidx roidx); subst; mred; [|eauto; fail].
+    specialize (H _ eq_refl); destruct H as [orq2 [? ?]].
+    exists orq2; split; [assumption|].
+    apply RssORqEquiv_addRs; assumption.
+  Qed.
+
+  Lemma findRs_putRs_eq:
+    forall midx rs rss,
+      In (midx, None) rss ->
+      findRs midx (putRs midx rs rss) = Some rs.
+  Proof.
+    induction rss as [|[rmidx irs]]; simpl; intros; [exfalso; auto|].
+    destruct H; subst; simpl in *.
+    - inv H.
+      destruct (idx_dec midx midx); [|exfalso; auto].
+      simpl; destruct (idx_dec midx midx); [|exfalso; auto].
+      reflexivity.
+    - destruct (idx_dec midx rmidx); subst.
+      + simpl; destruct (idx_dec rmidx rmidx); [reflexivity|exfalso; auto].
+      + simpl; destruct (idx_dec rmidx midx); [exfalso; auto|].
+        apply IHrss; assumption.
+  Qed.
+
+  Lemma findRs_putRs_neq:
+    forall midx amidx,
+      midx <> amidx ->
+      forall rs rss,
+        findRs midx (putRs amidx rs rss) = findRs midx rss.
+  Proof.
+    induction rss as [|[rmidx irs]]; simpl; intros; [reflexivity|].
+    destruct (idx_dec amidx rmidx); subst; simpl.
+    - destruct (idx_dec rmidx midx); subst; [exfalso; auto|reflexivity].
+    - destruct (idx_dec rmidx midx); subst; [reflexivity|assumption].
+  Qed.
+
+  Lemma SimRssMP_addRs:
+    forall iorqs imsgs smsgs,
+      SimRssMP iorqs imsgs smsgs ->
+      forall oidx porq,
+        iorqs@[oidx] = Some porq ->
+        forall rqid,
+          porq@[downRq] = Some rqid ->
+          RssWf oidx (rqi_rss rqid) ->
+          forall cidx,
+            parentIdxOf topo cidx = Some oidx ->
+            In (rsUpFrom cidx, None) (rqi_rss rqid) ->
+            forall rs,
+              FirstMP imsgs (rsUpFrom cidx) rs ->
+              SimRssMP (iorqs +[oidx <- addRs porq (rsUpFrom cidx) rs])
+                       (deqMP (rsUpFrom cidx) imsgs) smsgs.
+  Proof.
+    unfold SimRssMP; intros.
+    specialize (H midx); dest.
+    repeat split; intros.
+    1-2: rewrite findQ_not_In_deqMP by (intro Hx; rewrite Hx in H8; discriminate); eauto.
+
+    clear H H6.
+    subst midx.
+    specialize (H7 _ eq_refl _ H9 H10).
+    destruct (idx_dec oidx pidx); subst; mred;
+      [|rewrite findQ_not_In_deqMP by (intro Hx; inv Hx; congruence);
+        assumption].
+
+    simpl; unfold addRs.
+    rewrite H1; simpl; mred; simpl.
+    destruct (idx_dec oidx0 cidx); subst.
+    - rewrite findRs_putRs_eq by assumption.
+      simpl; rewrite findQ_In_deqMP_FirstMP by assumption.
+      erewrite findRs_rs in H7; [|apply H2|eassumption].
+      assumption.
+    - rewrite findRs_putRs_neq by (intro Hx; inv Hx; auto).
+      rewrite findQ_not_In_deqMP  by (intro Hx; inv Hx; auto).
+      assumption.
+  Qed.
+
+  Lemma SimRssMP_rss_full_first:
+    forall iorqs imsgs smsgs,
+      SimRssMP iorqs imsgs smsgs ->
+      forall oidx orq rqid,
+        In oidx (c_li_indices cifc ++ c_l1_indices cifc) ->
+        iorqs@[oidx] = Some orq ->
+        orq@[downRq] = Some rqid ->
+        NoDup (map fst (rqi_rss rqid)) ->
+        Forall (fun iom =>
+                  exists cidx,
+                    parentIdxOf topo cidx = Some oidx /\
+                    rsUpFrom cidx = fst iom) (rqi_rss rqid) ->
+        forall rss,
+          rqi_rss rqid = map (fun idm => (idOf idm, Some (valOf idm))) rss ->
+          Forall (FirstMPI smsgs) rss.
+  Proof.
+    unfold SimRssMP; intros.
+    apply Forall_forall; intros [rmidx rs] ?.
+    assert (In (rmidx, Some rs) (rqi_rss rqid))
+      by (rewrite H5; apply in_map_iff; eexists (_, _); simpl; eauto).
+
+    rewrite Forall_forall in H4; specialize (H4 _ H7).
+    destruct H4 as [cidx ?]; simpl in H4; dest; subst.
+    specialize (H (rsUpFrom cidx)); dest.
+    clear H H8.
+    specialize (H9 _ eq_refl _ H0 H4).
+    rewrite H1 in H9; simpl in H9.
+    rewrite H2 in H9; simpl in H9.
+
+    erewrite findRs_rs in H9 by eassumption.
+    simpl in H9.
+    unfold FirstMPI, FirstMP, firstMP.
+    simpl; rewrite <-H9.
+    reflexivity.
+  Qed.
+
+  Lemma RssORqEquiv_removeRq:
+    forall orq1 orq2,
+      RssORqEquiv orq1 orq2 ->
+      RssORqEquiv (removeRq orq1 downRq) (removeRq orq2 downRq).
+  Proof.
+    unfold RssORqEquiv, removeRq; intros; dest.
+    repeat split; mred.
+  Qed.
+
+  Lemma SimRssORqs_removeRq:
+    forall orqs1 orqs2,
+      SimRssORqs orqs1 orqs2 ->
+      forall roidx porq1 porq2,
+        orqs1@[roidx] = Some porq1 ->
+        orqs2@[roidx] = Some porq2 ->
+        SimRssORqs (orqs1+[roidx <- removeRq porq1 downRq])
+                   (orqs2+[roidx <- removeRq porq2 downRq]).
+  Proof.
+    unfold SimRssORqs, removeRq; intros.
+    rewrite Forall_forall in H.
+    apply Forall_forall; intros oidx ? ? ?.
+    specialize (H _ H2).
+    destruct (idx_dec oidx roidx); subst; mred; [|eauto; fail].
+    specialize (H _ eq_refl); destruct H as [orq2 [? ?]].
+    inv H.
+    eexists; split; [reflexivity|].
+    apply RssORqEquiv_removeRq; assumption.
+  Qed.
+
+  Lemma SimRssMP_removeRq:
+    forall iorqs imsgs smsgs,
+      SimRssMP iorqs imsgs smsgs ->
+      forall roidx,
+        (* In roidx (c_li_indices cifc ++ c_l1_indices cifc) -> *)
+        forall porq,
+          iorqs@[roidx] = Some porq ->
+          forall rqid,
+            porq@[downRq] = Some rqid ->
+            NoDup (idsOf (getRss porq)) ->
+            rqi_rss rqid = map (fun idm => (idOf idm, Some (valOf idm))) (getRss porq) ->
+            Forall
+              (fun iom =>
+                 exists cidx : IdxT,
+                   parentIdxOf topo cidx = Some roidx /\
+                   rsUpFrom cidx = fst iom) (rqi_rss rqid) ->
+            SimRssMP (iorqs +[roidx <- removeRq porq downRq])
+                     imsgs (deqMsgs (idsOf (getRss porq)) smsgs).
+  Proof.
+    unfold SimRssMP, removeRq; intros.
+    specialize (H midx); dest.
+
+    repeat split.
+    - clear H5 H6.
+      intros; subst; specialize (H _ eq_refl).
+      rewrite findQ_not_In_deqMsgs; [assumption|].
+      unfold getRss; rewrite H1; simpl.
+      clear -H4.
+      induction (rqi_rss rqid) as [|[rmidx rs]]; simpl in *; [auto|].
+      destruct rs as [rs|]; simpl in *.
+      + intro Hx; destruct Hx; subst.
+        * inv H4; simpl in *; dest; inv H0.
+        * inv H4; elim (IHl H3); assumption.
+      + inv H4; auto.
+    - clear H H6.
+      intros; subst; specialize (H5 _ eq_refl).
+      rewrite findQ_not_In_deqMsgs; [assumption|].
+      unfold getRss; rewrite H1; simpl.
+      clear -H4.
+      induction (rqi_rss rqid) as [|[rmidx rs]]; simpl in *; [auto|].
+      destruct rs as [rs|]; simpl in *.
+      + intro Hx; destruct Hx; subst.
+        * inv H4; simpl in *; dest; inv H0.
+        * inv H4; elim (IHl H3); assumption.
+      + inv H4; auto.
+
+    - clear H H5.
+      intros; subst; specialize (H6 _ eq_refl _ H5 H7).
+      destruct (idx_dec roidx pidx); subst; repeat (simpl in *; mred).
+      + destruct (in_dec idx_dec (rsUpFrom oidx) (idsOf (getRss porq))).
+        * assert (exists rs, findRs (rsUpFrom oidx) (rqi_rss rqid) = Some rs).
+          { unfold getRss in i, H3; rewrite H1 in i, H3; simpl in *.
+            clear -i H3.
+            induction (rqi_rss rqid) as [|[rmidx rs]]; simpl in *; [exfalso; auto|].
+            destruct rs as [rs|]; simpl in *.
+            { destruct i; subst.
+              { destruct (idx_dec _ _); [eauto|exfalso; auto]. }
+              { inv H3.
+                specialize (IHl H1 H); destruct IHl as [irs ?].
+                rewrite <-H1.
+                destruct (idx_dec _ _); eauto.
+              }
+            }
+            { exfalso; destruct (retRss l); discriminate. }
+          }
+          destruct H as [rs ?].
+          rewrite H in H6; simpl in H6.
+
+          apply findQ_In_NoDup_deqMsgs with (mp:= smsgs) in i;
+            [|eassumption|rewrite <-H6; discriminate]; dest.
+          rewrite <-H8 in H6; congruence.
+
+        * assert (findRs (rsUpFrom oidx) (rqi_rss rqid) = None).
+          { unfold getRss in n, H3; rewrite H1 in n, H3; simpl in *.
+            clear -n.
+            induction (rqi_rss rqid) as [|[rmidx rs]]; simpl in *; [reflexivity|].
+            destruct rs as [rs|]; simpl in *.
+            { destruct (idx_dec _ _); subst; [elim n; left; reflexivity|].
+              destruct (in_dec idx_dec (rsUpFrom oidx) (idsOf (retRss l))).
+              { elim n; right; assumption. }
+              { auto. }
+            }
+            { destruct (idx_dec _ _); [reflexivity|auto]. }
+          }
+          rewrite H in H6; simpl in H6.
+
+          rewrite findQ_not_In_deqMsgs by assumption.
+          assumption.
+
+      + rewrite H6.
+        rewrite findQ_not_In_deqMsgs; [reflexivity|].
+        unfold getRss; rewrite H1; simpl.
+        clear -H4 H7 n.
+        induction (rqi_rss rqid) as [|[rmidx rs]]; simpl in *; [auto|].
+        destruct rs as [rs|]; simpl in *.
+        * intro Hx; destruct Hx; subst.
+          { inv H4; simpl in *; dest.
+            inv H0; congruence.
+          }
+          { inv H4; elim (IHl H3); assumption. }
+        * inv H4; auto.
+  Qed.
+
+  Ltac disc_SimRssORqs obj :=
+    match goal with
+    | [H: SimRssORqs ?orqs _ |- _] =>
+      let Hs := fresh "H" in
+      pose proof H as Hs;
+      red in Hs; rewrite <-Hoinds in Hs;
+      rewrite Forall_forall in Hs;
+      specialize (Hs (obj_idx obj) ltac:(apply in_map; assumption));
+      match goal with
+      | [Horq: orqs@[obj_idx obj] = Some _ |- _] =>
+        specialize (Hs _ Horq);
+        let sorq := fresh "sorq" in
+        destruct Hs as [sorq ?]; dest
+      end
+    end.
+
+  Ltac disc_RssWfInv obj :=
+    match goal with
+    | [H: RssWfInv {| st_orqs := ?orqs |}, Horq: ?orqs@[obj_idx obj] = Some _ |- _] =>
+      let Hi := fresh "Hi" in
+      pose proof (H (obj_idx obj)) as Hi;
+      simpl in Hi; rewrite Horq in Hi; simpl in Hi
+    end.
+
+  Ltac disc_RssWfORq obj :=
+    match goal with
+    | [H: RssWfORq (obj_idx obj) ?orq, Horq: ?orq@[downRq] = Some _ |- _] =>
+      let Hwfo := fresh "Hwfo" in
+      let Hrsb := fresh "Hrsb" in
+      red in H; rewrite Horq in H; destruct H as [Hwfo Hrsb]
+    end.
+
+  Ltac disc_RssORqEquiv :=
+    match goal with
+    | [He: RssORqEquiv ?orq1 ?orq2 |- _] =>
+      let Hul := fresh "Hul" in
+      let Hdln := fresh "Hdln" in
+      let Hdls := fresh "Hdls" in
+      destruct He as [Hul [Hdln Hdls]];
+      try match goal with
+          | [Ho: orq1@[downRq] = Some _ |- _] =>
+            specialize (Hdls _ Ho);
+            let srqid := fresh "srqid" in
+            destruct Hdls as [srqid ?]; dest
+          end
+    end.
+
+  Theorem mesi_rss_sim_ok:
+    InvSim step_m step_m RssWfInv sim impl spec.
+  Proof.
+    red; intros.
+    rename H1 into Hwf. (* [RssWfInv ist1] *)
+    clear H3. (* [RssWfInv ist2] *)
+
+    inv H2;
+      [apply mesi_rss_sim_silent; assumption
+      |apply mesi_rss_sim_ext_in; assumption
+      |apply mesi_rss_sim_ext_out; assumption
+      |].
+
+    destruct sst1 as [soss1 sorqs1 smsgs1].
+    red in H0; simpl in H0; dest; subst.
+
+    move Hsr at bottom.
+    pose proof (Hsr _ H1) as [sobj [HsoIn [Hsoi Hsrr]]].
+    specialize (Hsrr rule) as [Hsrr1 Hsrr2].
+
+    pose proof (Hir _ H1) as [Hirr Hrst].
+    specialize (Hirr _ H3).
+    destruct Hirr as [|[|]].
+
+    - (*! Normal rules *)
+      clear Hrst Hsrr2.
+      specialize (Hsrr1 H3 H0).
+
+      disc_SimRssORqs obj.
+
+      (* Discharge [RssEquivRule] to get the transition for the spec. *)
+      pose proof H10.
+      apply (proj1 (proj2 H0)) in H15.
+      specialize (H15 _ H14).
+      destruct H15 as [sorq2 [? ?]].
+
+      do 2 eexists.
+      repeat ssplit; [reflexivity|..].
+
+      + econstructor.
+        1-4: eassumption.
+        { exact H13. }
+        { eapply SimRssMP_NoRsUpInputs_first; eauto.
+          apply H0 in H9; assumption.
+        }
+        { destruct H8; split; [|assumption].
+          rewrite Hsminds, Hserqs.
+          rewrite Himinds, Hierqs in H8.
+          assumption.
+        }
+        { eapply H0; eassumption. }
+        { eassumption. }
+        { destruct H11; split; [|assumption].
+          rewrite Hsminds, Hserss.
+          rewrite Himinds, Hierss in H11.
+          assumption.
+        }
+        { assumption. }
+        { reflexivity. }
+        { reflexivity. }
+
+      + red; simpl; repeat ssplit; [reflexivity|..].
+        * apply SimRssORqs_next_ord; auto.
+        * apply SimRssMP_enqMsgs.
+          apply SimRssMP_deqMsgs; [|apply H0 in H9; assumption].
+          eapply SimRssMP_ORqs_change_silent; try eassumption.
+          apply H0 in H10; assumption.
+
+    - (*! [RsRelease] *)
+      clear Hrst Hsrr1.
+      destruct H0 as [ridx [msgId [rqId [prec [trs ?]]]]]; subst rule.
+      specialize (Hsrr2 _ _ _ _ _ H3).
+
+      disc_SimRssORqs obj.
+      disc_RssWfInv obj.
+
+      (* Discharge precondition and transition *)
+      disc_rule_conds_ex.
+      destruct ins; [clear H7 H8 H9 H12|discriminate].
+      eapply RssFullWithId_spec in H16; [|eassumption].
+      destruct H16 as [rqid [? [rss [? [? [? ?]]]]]]; subst rss.
+      disc_RssWfORq obj.
+      disc_rule_conds_ex.
+      disc_RssORqEquiv.
+
+      eexists (RlblInt _ _ _ _); eexists.
+      repeat ssplit; [simpl; reflexivity|..].
+
+      + econstructor.
+        * eassumption.
+        * eassumption.
+        * reflexivity.
+        * rewrite <-Hsoi; eassumption.
+        * rewrite <-Hsoi; eassumption.
+        * red in Hwfo; dest.
+          eapply SimRssMP_rss_full_first; eauto.
+          { rewrite <-Hoinds.
+            apply in_map_iff; eauto.
+          }
+          { congruence. }
+          { congruence. }
+        * destruct H12; split; [|assumption].
+          rewrite Hierqs, Himinds in H12.
+          rewrite Hserqs, Hsminds; assumption.
+        * repeat split.
+          { red; rewrite H7; simpl.
+            rewrite <-H14, H8.
+            rewrite map_map; reflexivity.
+          }
+          { assumption. }
+          { red; rewrite H7; simpl.
+            rewrite <-H13, Hmsg; simpl; split; [assumption|reflexivity].
+          }
+          { red; rewrite H7; simpl.
+            rewrite <-H16, Hidx; simpl; auto.
+          }
+          { red; red in Hwfo; dest.
+            apply Forall_forall; intros [rmidx rs] ?; simpl.
+            apply in_map with (f:= fun idm => (idOf idm, Some (valOf idm))) in H22; simpl in H22.
+            rewrite Forall_forall in H21; specialize (H21 _ H22).
+            assumption.
+          }
+          { assumption. }
+
+        * simpl; unfold TrsMTrs, getDownLockMsg, getDownLockIdxBack; simpl.
+          rewrite H7; simpl.
+          rewrite <-H13, Hmsg, <-H16, Hidx; simpl.
+          reflexivity.
+        * destruct H11.
+          split; [|assumption].
+          rewrite Himinds, Hierss in H11.
+          rewrite Hsminds, Hserss; assumption.
+        * red in Hwfo; dest.
+          simpl; clear -H20 Hrsb.
+          apply (DisjList_false_spec idx_dec).
+          intros midx; intros; dest_in.
+          rewrite Forall_forall in H20.
+          apply in_map_iff in H; destruct H as [[rmidx rs] [? ?]]; simpl in *; subst.
+          apply in_map with (f:= fun idm => (idOf idm, Some (valOf idm))) in H0.
+          specialize (H20 _ H0).
+          destruct H20 as [cidx [? ?]]; simpl in *; subst.
+          elim (Hrsb cidx); reflexivity.
+        * reflexivity.
+        * reflexivity.
+
+      + red; simpl; repeat ssplit; [congruence|..].
+        * rewrite <-Hsoi.
+          apply SimRssORqs_removeRq; [assumption|assumption|congruence].
+        * eapply SimRssMP_enqMP.
+          eapply SimRssMP_removeRq; eauto.
+          { apply H12. }
+          { rewrite H8; apply Hwfo. }
+
+    - (*! [RsTakeOne] *)
+      clear Hrst Hsrr1 Hsrr2 Hrst.
+      destruct H0 as [ridx [msgId [rqId [cidx ?]]]]; dest; subst rule.
+      disc_SimRssORqs obj.
+      disc_rule_conds_ex.
+      disc_RssWfInv obj.
+      disc_RssWfORq obj.
+
+      exists RlblEmpty; eexists.
+      repeat ssplit; [reflexivity|constructor|].
+      red; simpl; repeat ssplit; [meq|..].
+      + apply SimRssORqs_addRs; auto.
+      + red in H18; rewrite Hrqi in H18; simpl in H18.
+        eapply SimRssMP_addRs; try eassumption.
+  Qed.
+
+  Hypothesis (HwfInv: InvReachable impl step_m RssWfInv).
+  Theorem mesi_ok:
+    (steps step_m) # (steps step_m) |-- impl ⊑ spec.
+  Proof.
+    eapply invRSim_implies_refinement with (sim:= sim).
+    - eassumption.
+    - apply mesi_rss_sim_init.
+    - apply mesi_rss_sim_ok.
+  Qed.
+
+End RssHolderOk.
